update and create new theorems. I now know other ways to prove goals Also simplify instructions back into state

Bar.lean
@@ -52,65 +52,63 @@ def Stack := List Frame
 deriving Repr
 
 inductive State where
-  | compute (ρ : List (String × Value)) (s : Stack) : State
-  | ret (s : Stack) : State
+  | compute (m: Term) (ρ : List (String × Value)) (s : Stack) : State
+  | ret (v: Value) (s : Stack) : State
   | error : State
-  | halt : State
+  | halt (v: Value) : State
 deriving Repr
 
-inductive Instruction where
-  | term (t: Term): Instruction
-  | value (v: Value): Instruction
 
 def lookup_var (e: List (String × Value)) (x: String) : Option Value :=
   match e with
   | []  => none
   | (y, v) :: e => if x == y then some v else lookup_var e x
 
--- inductive big_step : State -> State -> Prop
---   | computeLookup {x p s} :
---     big_step (State.compute (Term.var x) p s) (match lookup_var p x with | none => State.error | some v => State.ret v s)
---   | computeConstant {c p s} : big_step (State.compute (Term.con c) p s) (State.ret (Value.vCon c) s)
---   | computeLambda {x m p s} : big_step (State.compute (Term.lam x m) p s) (State.ret (Value.vLam x m p) s)
---   | computeDelay {m p s} : big_step (State.compute (Term.delay m) p s) (State.ret (Value.vDelay m p) s)
---   | computeForce {m p s} : big_step (State.compute (Term.force m) p s) (State.compute m p (Frame.force :: s))
---   | computeApp {m n p s} : big_step (State.compute (Term.app m n) p s) (State.compute m p (Frame.leftAppTerm n p :: s))
---   | computeBuiltin {b p s} : big_step (State.compute (Term.builtin b) p s) (State.ret (Value.vBuiltin (BuiltinValue.builtin b)) s)
---   | computeError {p s} : big_step (State.compute Term.error p s) State.error
---   | ret {v s} : big_step (State.ret v s) (State.halt v)
---   | retLeftAppTerm {m p v s} : big_step (State.ret v (Frame.leftAppTerm m p :: s)) (State.compute m p (Frame.rightApp v :: s))
---   | retRightApp {x m p v s} : big_step (State.ret v (Frame.rightApp (Value.vLam x m p) :: s)) (State.compute m ((x, v) :: p) s)
---   | retLeftAppValue {x m p v s} : big_step (State.ret (Value.vLam x m p) (Frame.leftAppValue v :: s)) (State.compute m ((x, v) :: p) s)
---   | retRightAppBuiltin {b v s} : big_step (State.ret v (Frame.rightApp (Value.vBuiltin b) :: s)) (State.ret (Value.vBuiltin (BuiltinValue.app b v)) s)
---   | retLeftAppValueBuiltin {b v s} : big_step (State.ret (Value.vBuiltin b) (Frame.leftAppValue v :: s)) (State.ret (Value.vBuiltin (BuiltinValue.app b v)) s)
---   | retDelay {m p s} : big_step (State.ret (Value.vDelay m p) (Frame.force :: s)) (State.compute m p s)
---   | retBuiltin {b s} : big_step (State.ret (Value.vBuiltin b) (Frame.force :: s)) (State.ret (Value.vBuiltin (BuiltinValue.force b)) s)
---   | catchAll {s} : big_step s State.error
+inductive small_step : State -> State -> Prop
+  | seq {s s' s''} (h: small_step s s') (h': small_step s' s''):
+    small_step s s''
+  | computeLookup {x p s} (h: lookup_var p x = some v): small_step (State.compute (Term.var x) p s) (State.ret v s)
+  | computeConstant {c p s} : small_step (State.compute (Term.con c) p s) (State.ret (Value.vCon c) s)
+  | computeLambda {x m p s} : small_step (State.compute (Term.lam x m) p s) (State.ret (Value.vLam x m p) s)
+  | computeDelay {m p s} : small_step (State.compute (Term.delay m) p s) (State.ret (Value.vDelay m p) s)
+  | computeForce {m p s} : small_step (State.compute (Term.force m) p s) (State.compute m p (Frame.force :: s))
+  | computeApp {m n p s} : small_step (State.compute (Term.app m n) p s) (State.compute m p (Frame.leftAppTerm n p :: s))
+  | computeBuiltin {b p s} : small_step (State.compute (Term.builtin b) p s) (State.ret (Value.vBuiltin (BuiltinValue.builtin b)) s)
+  | computeError {p s} : small_step (State.compute Term.error p s) State.error
+  | ret {v s} : small_step (State.ret v s) (State.halt v)
+  | retLeftAppTerm {m p v s} : small_step (State.ret v (Frame.leftAppTerm m p :: s)) (State.compute m p (Frame.rightApp v :: s))
+  | retRightApp {x m p v s} : small_step (State.ret v (Frame.rightApp (Value.vLam x m p) :: s)) (State.compute m ((x, v) :: p) s)
+  | retLeftAppValue {x m p v s} : small_step (State.ret (Value.vLam x m p) (Frame.leftAppValue v :: s)) (State.compute m ((x, v) :: p) s)
+  | retRightAppBuiltin {b v s} : small_step (State.ret v (Frame.rightApp (Value.vBuiltin b) :: s)) (State.ret (Value.vBuiltin (BuiltinValue.app b v)) s)
+  | retLeftAppValueBuiltin {b v s} : small_step (State.ret (Value.vBuiltin b) (Frame.leftAppValue v :: s)) (State.ret (Value.vBuiltin (BuiltinValue.app b v)) s)
+  | retDelay {m p s} : small_step (State.ret (Value.vDelay m p) (Frame.force :: s)) (State.compute m p s)
+  | retBuiltin {b s} : small_step (State.ret (Value.vBuiltin b) (Frame.force :: s)) (State.ret (Value.vBuiltin (BuiltinValue.force b)) s)
+  | catchAll {s} : small_step s State.error
 
-  inductive small_step : (Instruction × State) -> (Instruction × State) -> Prop
-  | seq {m m' m'' s s' s''} (h: small_step (m, s) (m', s')) (h': small_step (m', s') (m'', s'')):
-    small_step (m, s) (m'', s'')
+  -- inductive small_step : (Instruction × State) -> (Instruction × State) -> Prop
+  -- | seq {m m' m'' s s' s''} (h: small_step (m, s) (m', s')) (h': small_step (m', s') (m'', s'')):
+  --   small_step (m, s) (m'', s'')
 
-  | computeLookup {v x p s} :
-    small_step (Instruction.term (Term.var x), State.compute ((x, v) :: p) s) (Instruction.value v, State.ret s)
+  -- | computeLookup {v x p s} (h: lookup_var p x = some v):
+  --   small_step (Instruction.term (Term.var x), State.compute p s) (Instruction.value v, State.ret s)
 
-  | computeConstant {c p s} : small_step (Instruction.term (Term.con c) ,State.compute p s) (Instruction.value (Value.vCon c), State.ret s)
-  | computeLambda {x m p s} : small_step (Instruction.term (Term.lam x m), State.compute p s) (Instruction.value (Value.vLam x m p), State.ret s)
-  | computeDelay {m p s} : small_step (Instruction.term (Term.delay m), State.compute p s) (Instruction.value (Value.vDelay m p), State.ret s)
-  | computeForce {m p s} : small_step (Instruction.term (Term.force m), State.compute p s) (Instruction.term m, State.compute p (Frame.force :: s))
-  | computeApp {m n p s} : small_step (Instruction.term (Term.app m n), State.compute p s) (Instruction.term m, State.compute p (Frame.leftAppTerm n p :: s))
-  | computeBuiltin {b p s} : small_step (Instruction.term (Term.builtin b), State.compute  p s) (Instruction.value (Value.vBuiltin (BuiltinValue.builtin b)), State.ret s)
-  | computeError {p s} : small_step (Instruction.term Term.error, State.compute p s) (Instruction.term Term.error, State.error)
-  | ret {v} : small_step (Instruction.value v, State.ret []) (Instruction.value v, State.halt)
-  | retLeftAppTerm {m p v s} : small_step (Instruction.value v, State.ret (Frame.leftAppTerm m p :: s)) (Instruction.term m, State.compute p (Frame.rightApp v :: s))
-  | retRightApp {x m p v s} : small_step (Instruction.value v, State.ret (Frame.rightApp (Value.vLam x m p) :: s)) (Instruction.term m, State.compute ((x, v) :: p) s)
-  | retLeftAppValue {x m p v s} : small_step (Instruction.value (Value.vLam x m p), State.ret (Frame.leftAppValue v :: s)) (Instruction.term m, State.compute ((x, v) :: p) s)
-  | retRightAppBuiltin {b v s} : small_step (Instruction.value v, State.ret (Frame.rightApp (Value.vBuiltin b) :: s)) (Instruction.value (Value.vBuiltin (BuiltinValue.app b v)), State.ret s)
-  | retLeftAppValueBuiltin {b v s} : small_step (Instruction.value (Value.vBuiltin b), State.ret  (Frame.leftAppValue v :: s)) (Instruction.value (Value.vBuiltin (BuiltinValue.app b v)), State.ret s)
-  -- TODO: Eval builtins
-  | retDelay {m p s} : small_step (Instruction.value (Value.vDelay m p), State.ret (Frame.force :: s)) (Instruction.term m, State.compute p s)
-  | retBuiltin {b s} : small_step (Instruction.value (Value.vBuiltin b), State.ret (Frame.force :: s)) (Instruction.value (Value.vBuiltin (BuiltinValue.force b)), State.ret s)
-  | catchAll {m s} : small_step (m, s) ((Instruction.term Term.error), State.error)
+  -- | computeConstant {c p s} : small_step (Instruction.term (Term.con c) ,State.compute p s) (Instruction.value (Value.vCon c), State.ret s)
+  -- | computeLambda {x m p s} : small_step (Instruction.term (Term.lam x m), State.compute p s) (Instruction.value (Value.vLam x m p), State.ret s)
+  -- | computeDelay {m p s} : small_step (Instruction.term (Term.delay m), State.compute p s) (Instruction.value (Value.vDelay m p), State.ret s)
+  -- | computeForce {m p s} : small_step (Instruction.term (Term.force m), State.compute p s) (Instruction.term m, State.compute p (Frame.force :: s))
+  -- | computeApp {m n p s} : small_step (Instruction.term (Term.app m n), State.compute p s) (Instruction.term m, State.compute p (Frame.leftAppTerm n p :: s))
+  -- | computeBuiltin {b p s} : small_step (Instruction.term (Term.builtin b), State.compute  p s) (Instruction.value (Value.vBuiltin (BuiltinValue.builtin b)), State.ret s)
+  -- | computeError {p s} : small_step (Instruction.term Term.error, State.compute p s) (Instruction.term Term.error, State.error)
+  -- | ret {v} : small_step (Instruction.value v, State.ret []) (Instruction.value v, State.halt)
+  -- | retLeftAppTerm {m p v s} : small_step (Instruction.value v, State.ret (Frame.leftAppTerm m p :: s)) (Instruction.term m, State.compute p (Frame.rightApp v :: s))
+  -- | retRightApp {x m p v s} : small_step (Instruction.value v, State.ret (Frame.rightApp (Value.vLam x m p) :: s)) (Instruction.term m, State.compute ((x, v) :: p) s)
+  -- | retLeftAppValue {x m p v s} : small_step (Instruction.value (Value.vLam x m p), State.ret (Frame.leftAppValue v :: s)) (Instruction.term m, State.compute ((x, v) :: p) s)
+  -- | retRightAppBuiltin {b v s} : small_step (Instruction.value v, State.ret (Frame.rightApp (Value.vBuiltin b) :: s)) (Instruction.value (Value.vBuiltin (BuiltinValue.app b v)), State.ret s)
+  -- | retLeftAppValueBuiltin {b v s} : small_step (Instruction.value (Value.vBuiltin b), State.ret  (Frame.leftAppValue v :: s)) (Instruction.value (Value.vBuiltin (BuiltinValue.app b v)), State.ret s)
+  -- -- TODO: Eval builtins
+  -- | retDelay {m p s} : small_step (Instruction.value (Value.vDelay m p), State.ret (Frame.force :: s)) (Instruction.term m, State.compute p s)
+  -- | retBuiltin {b s} : small_step (Instruction.value (Value.vBuiltin b), State.ret (Frame.force :: s)) (Instruction.value (Value.vBuiltin (BuiltinValue.force b)), State.ret s)
+  -- | catchAll {m s} : small_step (m, s) ((Instruction.term Term.error), State.error)
 
 
 infix: 90 "⟶" => small_step
@@ -118,82 +116,134 @@ infix: 90 "⟶" => small_step
 
 
 theorem small_step_compute_lambda
-{x m p s} : (Instruction.term (Term.lam x m), State.compute  p s) ⟶ (Instruction.value (Value.vLam x m p), State.ret s) := by
+{x m p s} : (State.compute (Term.lam x m) p s) ⟶ (State.ret (Value.vLam x m p) s) := by
   apply small_step.computeLambda
+
+
+theorem frame_force_delay_just_term
+  {m p s}:
+  (State.compute (Term.delay m) p (Frame.force :: s)) ⟶
+  (State.compute m p s) := by
+    have h': (State.compute (Term.delay m) p (Frame.force :: s)) ⟶
+      (State.ret (Value.vDelay m p) (Frame.force :: s)) := by
+        apply small_step.computeDelay
+    have h'': (State.ret (Value.vDelay m p) (Frame.force :: s)) ⟶
+      (State.compute m p s) := by
+        apply small_step.retDelay
+    exact small_step.seq h' h''
+
+theorem forcing
+  {m p s}:
+  (State.compute (Term.force (Term.force m)) p (s)) ⟶
+  (State.compute m p (Frame.force :: Frame.force :: s)) := by
+    exact small_step.seq small_step.computeForce small_step.computeForce
 
 
 theorem force_delay_just_term
   {m p s}:
-  (Instruction.term (Term.force (Term.delay m)), State.compute p s) ⟶
-  (Instruction.term m, State.compute p s) := by
-    have h: (Instruction.term (Term.force (Term.delay m)), State.compute p s) ⟶
-      (Instruction.term (Term.delay m), State.compute p (Frame.force :: s)) := by
+  (State.compute (Term.force (Term.delay m)) p s) ⟶
+  (State.compute m p s) := by
+    have h: (State.compute (Term.force (Term.delay m)) p s) ⟶
+      (State.compute (Term.delay m) p (Frame.force :: s)) := by
         apply small_step.computeForce
-    have h': (Instruction.term (Term.delay m), State.compute p (Frame.force :: s)) ⟶
-      (Instruction.value (Value.vDelay m p), State.ret (Frame.force :: s)) := by
+    have h': (State.compute (Term.delay m) p (Frame.force :: s)) ⟶
+      (State.ret (Value.vDelay m p) (Frame.force :: s)) := by
         apply small_step.computeDelay
-    have h'': (Instruction.value (Value.vDelay m p), State.ret (Frame.force :: s)) ⟶
-      (Instruction.term m, State.compute p s) := by
+    have h'': (State.ret (Value.vDelay m p) (Frame.force :: s)) ⟶
+      (State.compute m p s) := by
         apply small_step.retDelay
     exact small_step.seq (small_step.seq h h') h''
 
+theorem double_force_term
+  {m p s}:
+  (State.compute (Term.force (Term.force m)) p s) ⟶
+  (State.compute m p (Frame.force :: Frame.force :: s)) := by
+    have h: (State.compute (Term.force (Term.force m)) p s) ⟶
+      (State.compute (Term.force m) p (Frame.force :: s)) := by
+        apply small_step.computeForce
+    let s' := Frame.force :: s
+    have h': (State.compute (Term.force m) p s') ⟶
+      (State.compute m p (Frame.force :: s')) := by
+        apply small_step.computeForce
+    exact small_step.seq h h'
+
+theorem force_delay_term
+  {m p s}:
+  (State.compute (Term.force (Term.force (Term.delay (Term.delay m)))) p s) ⟶
+  (State.compute m p s) := by
+    have h: (State.compute (Term.force (Term.force (Term.delay (Term.delay m)))) p s) ⟶
+      (State.compute (Term.force (Term.delay (Term.delay m))) p (Frame.force :: s)) := by
+        apply small_step.computeForce
+    have h': (State.compute (Term.force (Term.delay (Term.delay m))) p (Frame.force :: s)) ⟶
+      (State.compute (Term.delay m) p (Frame.force :: s)) := by
+        exact force_delay_just_term
+    have h'': (State.compute (Term.delay m) p (Frame.force :: s)) ⟶
+      (State.compute m p s) := by
+        apply frame_force_delay_just_term
+    exact small_step.seq (small_step.seq h h') h''
+
+theorem forces
+  {m p s}:
+  (State.compute (Term.force (Term.force (Term.force (Term.delay (Term.delay (Term.delay m)))))) p s) ⟶
+  (State.compute m p s) := by
+    apply small_step.seq
+    case h =>
+      apply small_step.seq
+      case h => exact forcing
+      case h' => exact force_delay_just_term
+    case h' =>
+      apply small_step.seq
+      case h => exact frame_force_delay_just_term
+      case h' => exact frame_force_delay_just_term
+
+theorem forces2
+  {m p s}:
+  (State.compute (Term.force (Term.force (Term.force (Term.delay (Term.delay (Term.delay m)))))) p s) ⟶
+  (State.compute m p s) := by
+    repeat (
+      first
+      | apply forcing
+      | apply force_delay_just_term
+      | apply frame_force_delay_just_term
+      | apply small_step.seq
+    )
 
 
-theorem lam_apply_var_is_applied_term
-  {x p s}:
-  (Instruction.term (Term.app (Term.lam x (Term.var x)) (Term.con 5)), State.compute p s) ⟶
-  (Instruction.value (Value.vCon 5), State.ret s) := by
-    have h: (Instruction.term (Term.app (Term.lam x (Term.var x)) (Term.con 5)), State.compute p s) ⟶
-      (Instruction.term (Term.lam x (Term.var x)), State.compute p (Frame.leftAppTerm (Term.con 5) p :: s)) := by
-        apply small_step.computeApp
-    have h': (Instruction.term (Term.lam x (Term.var x)), State.compute p (Frame.leftAppTerm (Term.con 5) p :: s)) ⟶
-      (Instruction.value (Value.vLam x (Term.var x) p), State.ret (Frame.leftAppTerm (Term.con 5) p :: s)) := by
-        apply small_step.computeLambda
-    have h'': (Instruction.value (Value.vLam x (Term.var x) p), State.ret (Frame.leftAppTerm (Term.con 5) p :: s)) ⟶
-      (Instruction.term (Term.con 5), State.compute p ((Frame.rightApp (Value.vLam x (Term.var x) p)) :: s)) := by
-        apply small_step.retLeftAppTerm
-    have h''': (Instruction.term (Term.con 5), State.compute p ((Frame.rightApp (Value.vLam x (Term.var x) p)) :: s)) ⟶
-      (Instruction.value (Value.vCon 5), State.ret ((Frame.rightApp (Value.vLam x (Term.var x) p)) :: s)) := by
-        apply small_step.computeConstant
-    have h'''': (Instruction.value (Value.vCon 5), State.ret ((Frame.rightApp (Value.vLam x (Term.var x) p)) :: s)) ⟶
-      (Instruction.term (Term.var x), State.compute ((x, (Value.vCon 5)) :: p) s) := by
-        apply small_step.retRightApp
-    have h''''' : (Instruction.term (Term.var x), State.compute ((x, (Value.vCon 5)) :: p) s) ⟶
-      (Instruction.value (Value.vCon 5), State.ret s) := by
-        apply small_step.computeLookup
-    exact small_step.seq (small_step.seq (small_step.seq (small_step.seq (small_step.seq h h') h'') h''') h'''') h'''''
+theorem forces3
+  {m p s}:
+  (State.compute (Term.force (Term.force (Term.force (Term.delay (Term.delay (Term.delay m)))))) p s) ⟶
+  (State.compute m p s) := by
+    repeat (first | apply small_step.computeForce | apply small_step.computeDelay | apply small_step.retDelay | apply small_step.seq)
 
 
 
--- partial def reduc (st : State) : State :=
---   match st with
---   | State.compute (Term.var x) ρ s => match lookup_var ρ x with
---     | none => State.error
---     | some v => reduc (State.ret v s)
---   | State.compute (Term.con c) _ s => reduc (State.ret (Value.vCon c) s)
---   | State.compute (Term.lam x m) ρ s => reduc (State.ret (Value.vLam x m ρ) s)
---   | State.compute (Term.delay m) ρ s => reduc (State.ret (Value.vDelay m ρ) s)
---   | State.compute (Term.force m) ρ s => reduc (State.compute m ρ (Frame.force :: s))
---   | State.compute (Term.app m n) p s => reduc (State.compute m p (Frame.leftAppTerm n p :: s))
---   | State.compute (Term.builtin b) _ s => reduc (State.ret (Value.vBuiltin (BuiltinValue.builtin b)) s)
---   | State.compute Term.error _ _ => State.error
---   | State.ret v [] => State.halt v
---   | State.ret v (Frame.leftAppTerm m p :: s) => reduc (State.compute m p (Frame.rightApp v :: s))
---   | State.ret v (Frame.rightApp (Value.vLam x m p) :: s) => reduc (State.compute m ((x, v) :: p) s)
---   | State.ret (Value.vLam x m p) (Frame.leftAppValue v :: s) => reduc (State.compute m ((x, v) :: p) s)
---   | State.ret v (Frame.rightApp (Value.vBuiltin b) :: s) => reduc (State.ret (Value.vBuiltin (BuiltinValue.app b v)) s)
---   | State.ret (Value.vBuiltin b) (Frame.leftAppValue v :: s) => reduc (State.ret (Value.vBuiltin (BuiltinValue.app b v)) s)
---   -- TODO: Eval builtins
---   | State.ret (Value.vDelay m p) (Frame.force :: s) => reduc (State.compute m p s)
---   | State.ret (Value.vBuiltin b) (Frame.force :: s) => reduc (State.ret (Value.vBuiltin (BuiltinValue.force b)) s)
---   | _ => State.error
-
--- def run (p: Program) : State :=
---   reduc (State.compute p.m [] [])
-
--- def test2 : State :=
---   let x := run ({v := 0, m := Term.app (Term.lam "so" (Term.var "so")) (Term.con 5)})
---   x
+-- theorem lam_apply_var_is_applied_term
+--   {x p s}:
+--   (Instruction.term (Term.app (Term.lam x (Term.var x)) (Term.con 5)), State.compute p s) ⟶
+--   (Instruction.value (Value.vCon 5), State.ret s) := by
+--     have h: (Instruction.term (Term.app (Term.lam x (Term.var x)) (Term.con 5)), State.compute p s) ⟶
+--       (Instruction.term (Term.lam x (Term.var x)), State.compute p (Frame.leftAppTerm (Term.con 5) p :: s)) := by
+--         apply small_step.computeApp
+--     have h': (Instruction.term (Term.lam x (Term.var x)), State.compute p (Frame.leftAppTerm (Term.con 5) p :: s)) ⟶
+--       (Instruction.value (Value.vLam x (Term.var x) p), State.ret (Frame.leftAppTerm (Term.con 5) p :: s)) := by
+--         apply small_step.computeLambda
+--     have h'': (Instruction.value (Value.vLam x (Term.var x) p), State.ret (Frame.leftAppTerm (Term.con 5) p :: s)) ⟶
+--       (Instruction.term (Term.con 5), State.compute p ((Frame.rightApp (Value.vLam x (Term.var x) p)) :: s)) := by
+--         apply small_step.retLeftAppTerm
+--     have h''': (Instruction.term (Term.con 5), State.compute p ((Frame.rightApp (Value.vLam x (Term.var x) p)) :: s)) ⟶
+--       (Instruction.value (Value.vCon 5), State.ret ((Frame.rightApp (Value.vLam x (Term.var x) p)) :: s)) := by
+--         apply small_step.computeConstant
+--     have h'''': (Instruction.value (Value.vCon 5), State.ret ((Frame.rightApp (Value.vLam x (Term.var x) p)) :: s)) ⟶
+--       (Instruction.term (Term.var x), State.compute ((x, (Value.vCon 5)) :: p) s) := by
+--         apply small_step.retRightApp
+--     have h''''' : (Instruction.term (Term.var x), State.compute ((x, (Value.vCon 5)) :: p) s) ⟶
+--       (Instruction.value (Value.vCon 5), State.ret s) := by
+--         apply small_step.computeLookup
+--     exact small_step.seq (small_step.seq (small_step.seq (small_step.seq (small_step.seq h h') h'') h''') h'''') h'''''
 
 
--- #eval test2
+theorem lam_apply_var_is_applied_term2
+  {x p}:
+  (State.compute (Term.app (Term.lam x (Term.var x)) (Term.con 5)) p []) ⟶
+  (State.halt (Value.vCon 5)) := by
+    repeat (first | apply small_step.computeApp | apply small_step.computeLambda | apply small_step.retLeftAppTerm | apply small_step.computeConstant | apply small_step.retRightApp | apply small_step.computeLookup | apply small_step.ret | apply small_step.seq)
